isabella.ml/src/canon/confidential_transaction.ml
@@ -29,6 +29,11 @@ type membership_proof = {
 let make_membership_proof member_index member_root member_siblings member_directions =
   { member_index; member_root; member_siblings; member_directions }
 
+type merkle_membership_proof = Confidential_merkle.membership_proof
+
+let make_merkle_membership_proof merkle_index merkle_root merkle_siblings merkle_directions =
+  { Confidential_merkle.merkle_index; merkle_root; merkle_siblings; merkle_directions }
+
 type verified_note = {
   note_commitment : int list;
   note_range_proof : range_proof;
@@ -62,7 +67,35 @@ let make_transaction_proof
     tx_in2_nullifier;
     tx_balance;
     tx_out1_range;
-    tx_out2_range;
+      tx_out2_range;
+  }
+
+type merkle_transaction_proof = {
+  tx_merkle_in1_member : merkle_membership_proof;
+  tx_merkle_in2_member : merkle_membership_proof;
+  tx_merkle_in1_nullifier : nullifier_proof;
+  tx_merkle_in2_nullifier : nullifier_proof;
+  tx_merkle_balance : balance_proof;
+  tx_merkle_out1_range : range_proof;
+  tx_merkle_out2_range : range_proof;
+}
+
+let make_merkle_transaction_proof
+    tx_merkle_in1_member
+    tx_merkle_in2_member
+    tx_merkle_in1_nullifier
+    tx_merkle_in2_nullifier
+    tx_merkle_balance
+    tx_merkle_out1_range
+    tx_merkle_out2_range =
+  {
+    tx_merkle_in1_member;
+    tx_merkle_in2_member;
+    tx_merkle_in1_nullifier;
+    tx_merkle_in2_nullifier;
+    tx_merkle_balance;
+    tx_merkle_out1_range;
+    tx_merkle_out2_range;
   }
 
 let valid_commitment p c =
@@ -268,6 +301,21 @@ let membership_verify p c proof =
     index_directions (List.length proof.member_siblings) proof.member_index &&
   auth_path_root p c proof.member_siblings proof.member_directions = proof.member_root
 
+let merkle_ledger_root ledger =
+  Confidential_merkle.root ledger
+
+let merkle_membership_prove ledger c =
+  Confidential_merkle.membership_prove ledger c
+
+let merkle_membership_verify c proof =
+  Confidential_merkle.membership_verify c proof
+
+let merkle_member_root proof =
+  proof.Confidential_merkle.merkle_root
+
+let merkle_member_index proof =
+  proof.Confidential_merkle.merkle_index
+
 let commitment_ledger notes =
   List.map (fun note -> note.note_commitment) notes
 
@@ -279,6 +327,22 @@ let ledger_valid p gamma k ck root notes spent =
   Confidential_balance.valid_scalar_commit_params p &&
   Commit_sis.valid_commit_key p ck &&
   root = ledger_root p (commitment_ledger notes) &&
+  distinct spent &&
+  List.for_all
+    (fun note ->
+       Confidential_range.range_fs_verify
+         p
+         gamma
+         k
+         ck
+         note.note_commitment
+         note.note_range_proof)
+    notes
+
+let ledger_valid_merkle p gamma k ck root notes spent =
+  Confidential_balance.valid_scalar_commit_params p &&
+  Commit_sis.valid_commit_key p ck &&
+  root = merkle_ledger_root (commitment_ledger notes) &&
   distinct spent &&
   List.for_all
     (fun note ->
@@ -345,6 +409,28 @@ let transaction_fs_verify p gamma k ck nk root spent c_in1 c_in2 c_out1 c_out2 n
   Confidential_range.range_fs_verify p gamma k ck c_out1 proof.tx_out1_range &&
   Confidential_range.range_fs_verify p gamma k ck c_out2 proof.tx_out2_range
 
+let transaction_fs_verify_merkle p gamma k ck nk root spent c_in1 c_in2 c_out1 c_out2 nf1 nf2 proof =
+  Commit_sis.valid_commit_key p ck &&
+  Commit_sis.valid_commit_key p nk &&
+  merkle_membership_verify c_in1 proof.tx_merkle_in1_member &&
+  merkle_membership_verify c_in2 proof.tx_merkle_in2_member &&
+  merkle_member_root proof.tx_merkle_in1_member = root &&
+  merkle_member_root proof.tx_merkle_in2_member = root &&
+  merkle_member_index proof.tx_merkle_in1_member <> merkle_member_index proof.tx_merkle_in2_member &&
+  not (List.mem nf1 spent) &&
+  not (List.mem nf2 spent) &&
+  nf1 <> nf2 &&
+  nullifier_fs_verify p gamma ck nk c_in1 nf1 proof.tx_merkle_in1_nullifier &&
+  nullifier_fs_verify p gamma ck nk c_in2 nf2 proof.tx_merkle_in2_nullifier &&
+  Confidential_balance.balance_fs_verify
+    p
+    gamma
+    ck
+    (Confidential_balance.balance_commitment c_in1 c_in2 c_out1 c_out2 p.Commit_sis.cp_q)
+    proof.tx_merkle_balance &&
+  Confidential_range.range_fs_verify p gamma k ck c_out1 proof.tx_merkle_out1_range &&
+  Confidential_range.range_fs_verify p gamma k ck c_out2 proof.tx_merkle_out2_range
+
 let transaction_fs_prove p gamma k ck nk ledger spent c_in1 c_in2 c_out1 c_out2 nf1 nf2
     op_in1 op_in2 op_out1 op_out2 out1_bits out1_comps out2_bits out2_comps
     y_in1 y_in2 y_balance y_out1 y_out1_pairs y_out2 y_out2_pairs =
@@ -380,6 +466,41 @@ let transaction_fs_prove p gamma k ck nk ledger spent c_in1 c_in2 c_out1 c_out2 
       else None
   | _ -> None
 
+let transaction_fs_prove_merkle p gamma k ck nk ledger spent c_in1 c_in2 c_out1 c_out2 nf1 nf2
+    op_in1 op_in2 op_out1 op_out2 out1_bits out1_comps out2_bits out2_comps
+    y_in1 y_in2 y_balance y_out1 y_out1_pairs y_out2 y_out2_pairs =
+  match
+    merkle_membership_prove ledger c_in1,
+    merkle_membership_prove ledger c_in2,
+    nullifier_fs_prove p gamma ck nk c_in1 nf1 op_in1 y_in1,
+    nullifier_fs_prove p gamma ck nk c_in2 nf2 op_in2 y_in2,
+    Confidential_balance.balance_fs_prove
+      p
+      gamma
+      ck
+      (Confidential_balance.balance_commitment c_in1 c_in2 c_out1 c_out2 p.Commit_sis.cp_q)
+      (Confidential_balance.aggregate_randomness op_in1 op_in2 op_out1 op_out2)
+      y_balance,
+    Confidential_range.range_fs_prove p gamma k ck c_out1 op_out1 out1_bits out1_comps y_out1 y_out1_pairs,
+    Confidential_range.range_fs_prove p gamma k ck c_out2 op_out2 out2_bits out2_comps y_out2 y_out2_pairs
+  with
+  | Some member1, Some member2, Some nf_proof1, Some nf_proof2, Some bal_proof, Some range1, Some range2 ->
+      if transaction_relation_wellformed p ck nk ledger spent c_in1 c_in2 c_out1 c_out2 nf1 nf2
+           op_in1 op_in2 op_out1 op_out2 out1_bits out1_comps out2_bits out2_comps &&
+         merkle_member_index member1 <> merkle_member_index member2
+      then
+        Some
+          (make_merkle_transaction_proof
+             member1
+             member2
+             nf_proof1
+             nf_proof2
+             bal_proof
+             range1
+             range2)
+      else None
+  | _ -> None
+
 let ledger_note_at notes proof =
   List.nth notes proof.member_index
 
@@ -395,6 +516,17 @@ let ledger_apply_notes notes proof c_out1 c_out2 =
   let out2 = make_verified_note c_out2 proof.tx_out2_range in
   out1 :: out2 :: remaining
 
+let ledger_note_at_merkle notes proof =
+  List.nth notes (merkle_member_index proof)
+
+let ledger_apply_notes_merkle notes proof c_out1 c_out2 =
+  let note1 = ledger_note_at_merkle notes proof.tx_merkle_in1_member in
+  let note2 = ledger_note_at_merkle notes proof.tx_merkle_in2_member in
+  let remaining = remove1 note2 (remove1 note1 notes) in
+  let out1 = make_verified_note c_out1 proof.tx_merkle_out1_range in
+  let out2 = make_verified_note c_out2 proof.tx_merkle_out2_range in
+  out1 :: out2 :: remaining
+
 let ledger_apply_spent spent nf1 nf2 =
   nf1 :: nf2 :: spent
 
@@ -408,3 +540,14 @@ let ledger_step_valid p gamma k ck nk notes spent c_in1 c_in2 c_out1 c_out2 nf1 
   ledger_valid p gamma k ck post_root updated_notes updated_spent
 
 let semantic_step_valid = ledger_step_valid
+
+let ledger_step_valid_merkle p gamma k ck nk notes spent c_in1 c_in2 c_out1 c_out2 nf1 nf2 proof =
+  let pre_root = merkle_ledger_root (commitment_ledger notes) in
+  let updated_notes = ledger_apply_notes_merkle notes proof c_out1 c_out2 in
+  let updated_spent = ledger_apply_spent spent nf1 nf2 in
+  let post_root = merkle_ledger_root (commitment_ledger updated_notes) in
+  ledger_valid_merkle p gamma k ck pre_root notes spent &&
+  transaction_fs_verify_merkle p gamma k ck nk pre_root spent c_in1 c_in2 c_out1 c_out2 nf1 nf2 proof &&
+  ledger_valid_merkle p gamma k ck post_root updated_notes updated_spent
+
+let semantic_step_valid_merkle = ledger_step_valid_merkle
